notation tweaks and stack proofs

src/stack_ra.v
@@ -1,5 +1,8 @@
 (* ghost state for environments *)
 From iris.algebra Require Import excl auth gmap.
+From iris.base_logic Require Import own.
+From iris.bi Require Export monpred.
+From iris.proofmode Require Export proofmode.
 From iris_simp_lang Require Import implang.
 
 Definition env_state := (gmap nat (gmap string val))%type.
@@ -14,6 +17,13 @@ Class envGS Σ := EnvGS {
   envGS_inG :: inG Σ envR;
   env_name : gname
 }.
+
+(* assertions are monPreds on stack level *)
+Definition stack_index : biIndex := {| bi_index_type := nat; bi_index_rel := eq |}.
+
+Definition assert `{!envGS Σ} := monPred stack_index (iPropI Σ).
+
+Program Definition assert_of `{!envGS Σ} (P : nat -> iProp Σ) : assert := {| monPred_at := P |}.
 
 Section env.
 
@@ -40,78 +50,71 @@ Qed.
 Definition stack_frag n q0 q r := own(inG0 := envGS_inG) env_name (◯ {[n := (to_agree q0, (q, (Excl <$> r)))]}).
 
 Definition points_to_var (id : string) (v : val) :=
-  assert_of (λ n, ∃ q, stack_frag n q q {[id := v]}).
+  assert_of (λ n, ∃ q, stack_frag n q q {[id := v]})%I.
+
+Definition env_to_environ (ρ : env_state) n : gmap string val :=
+  match ρ !! n with Some r => r | None => ∅ end.
 
 Lemma stack_frag_e' : forall ρ n q0 q r, env_auth ρ ∗ stack_frag n q0 q r ⊢
   ⌜let rho := env_to_environ ρ n in q0 = Qp.inv (pos_to_Qp (Pos.of_nat (1 + size rho))) ∧ r ⊆ rho⌝.
 Proof.
   intros; rewrite /env_auth /stack_frag.
-  iIntros "(H1 & H2)"; iDestruct (own_valid_2 with "H1 H2") as %(_ & ((? & Heq & H)%gmap.singleton_included_l & _)%auth_both_valid_discrete); iPureIntro.
-  rewrite lookup_fmap in Heq; rewrite /env_to_environ. destruct (snd ρ !! n)%stdpp as [(?, ?)|] eqn: Hn; rewrite !Hn in Heq |- *; inversion Heq as [?? HA |]; subst.
+  iIntros "(H1 & H2)"; iDestruct (own_valid_2 with "H1 H2") as %((? & Heq & H)%gmap.singleton_included_l & _)%auth_both_valid_discrete; iPureIntro.
+  rewrite lookup_fmap in Heq; rewrite /env_to_environ. destruct (ρ !! n) as [?|] eqn: Hn; rewrite !Hn in Heq |- *; inversion Heq as [?? HA |]; subst.
   rewrite -HA in H; clear Heq.
-  apply Some_included in H as [(? & ? & Hv & Ht) | ?]; simpl in *.
+  apply Some_included in H as [(? & ? & Hr) | ?]; simpl in *.
   - apply to_agree_inj in H.
-    apply (map_fmap_equiv_inj Excl), leibniz_equiv in Hv as ->; last apply Excl_inj.
-    apply (map_fmap_equiv_inj Excl), leibniz_equiv in Ht as ->; last apply Excl_inj; done.
-  - apply prod_included in H as (Hq & H); apply prod_included in H as (_ & H); apply prod_included in H as (Hv & Ht); simpl in *.
+    apply (map_fmap_equiv_inj Excl), leibniz_equiv in Hr as ->; last apply Excl_inj; done.
+  - apply prod_included in H as (Hq & H); apply prod_included in H as (_ & Hr); simpl in *.
     apply to_agree_included_L in Hq; split; first done.
-    rewrite !gmap.lookup_included in Hv Ht; split; intros i.
-    + specialize (Hv i); rewrite !lookup_fmap in Hv.
-      apply (Excl_fmap_incl(A := leibnizO _)) in Hv.
-      destruct (ve !! i)%stdpp.
-      * apply leibniz_equiv in Hv; rewrite -Hv //.
-      * simpl; clear; destruct (_ !! _)%stdpp; done.
-    + specialize (Ht i); rewrite !lookup_fmap in Ht.
-      apply (Excl_fmap_incl(A := leibnizO _)) in Ht.
-      destruct (te !! i)%stdpp.
-      * apply leibniz_equiv in Ht; rewrite -Ht //.
-      * simpl; clear; destruct (_ !! _)%stdpp; done.
+    rewrite !gmap.lookup_included in Hr; intros i.
+    specialize (Hr i); rewrite !lookup_fmap in Hr.
+    apply (Excl_fmap_incl(A := leibnizO _)) in Hr.
+    destruct (r !! i).
+    * apply leibniz_equiv in Hr; rewrite -Hr //.
+    * simpl; clear; destruct (_ !! _); done.
 Qed.
 
 Lemma stack_frag_e : forall ρ n q0 q r, env_auth ρ ∗ stack_frag n q0 q r ⊢
   ⌜let rho := env_to_environ ρ n in r ⊆ rho⌝.
 Proof.
-  intros; rewrite stack_frag_e'; apply bi.pure_mono; tauto.
+  intros; rewrite stack_frag_e'; apply bi.pure_mono; by intros (? & ?).
 Qed.
 
 Lemma stack_frag_e_1 : forall ρ n q0 r, env_auth ρ ∗ stack_frag n q0 1%Qp r ⊢
   ⌜let rho := env_to_environ ρ n in r = rho⌝.
 Proof.
   intros; rewrite /env_auth /stack_frag.
-  iIntros "(H1 & H2)"; iDestruct (own_valid_2 with "H1 H2") as %(_ & (H & Hvalid)%auth_both_valid_discrete).
+  iIntros "(H1 & H2)"; iDestruct (own_valid_2 with "H1 H2") as %(H & Hvalid)%auth_both_valid_discrete.
   apply gmap.singleton_included_exclusive_l in H; [| apply _ | done].
-  rewrite lookup_fmap in H; rewrite /env_to_environ. destruct (snd ρ !! n)%stdpp as [(?, ?)|] eqn: Hn; rewrite !Hn in H |- *; inversion H as [?? HA |]; subst.
-  destruct HA as (_ & _ & Hv & Ht); simpl in *.
-  apply (map_fmap_equiv_inj Excl), leibniz_equiv in Hv as ->; last apply Excl_inj.
-  apply (map_fmap_equiv_inj Excl), leibniz_equiv in Ht as ->; last apply Excl_inj; done.
+  rewrite lookup_fmap in H; rewrite /env_to_environ. destruct (ρ !! n) as [?|] eqn: Hn; rewrite !Hn in H |- *; inversion H as [?? HA |]; subst.
+  destruct HA as (_ & _ & Hr); simpl in *.
+  apply (map_fmap_equiv_inj Excl), leibniz_equiv in Hr as ->; last apply Excl_inj; done.
 Qed.
 
 Lemma var_e : forall id v rho n, points_to_var id v n ∗ env_auth rho ⊢ ⌜(env_to_environ rho n) !! id = Some v⌝.
 Proof.
-  intros; rewrite /temp /=.
-  iIntros "((% & ?) & ?)"; iDestruct (stack_frag_e with "[$]") as %(_ & ?%map_singleton_subseteq_l); done.
+  intros; rewrite /points_to_var /=.
+  iIntros "((% & ?) & ?)"; iDestruct (stack_frag_e with "[$]") as %?%map_singleton_subseteq_l; done.
 Qed.
 
-Definition set_temp (ρ : env_state) n i v :=
+Definition set_var (ρ : env_state) n i v :=
   match (ρ !! n)%stdpp with
   | Some r => <[n := <[i := v]>r]>ρ
   | None => ρ end.
 
-Lemma var_update : forall ρ n i v v', env_auth ρ ∗ points_to_var i v n ⊢ |==> env_auth (set_temp ρ n i v') ∗ points_to_var i v' n.
+Lemma var_update : forall ρ n i v v', env_auth ρ ∗ points_to_var i v n ⊢ |==> env_auth (set_var ρ n i v') ∗ points_to_var i v' n.
 Proof.
   intros.
   iIntros "(Hr & Hi)".
-  iDestruct (temp_e with "[$Hr $Hi]") as %Hi.
+  iDestruct (var_e with "[$Hr $Hi]") as %Hi.
   rewrite /env_to_environ in Hi.
-  destruct (snd ρ !! n)%stdpp as [(?, te)|] eqn: Hn; rewrite Hn in Hi; last by rewrite lookup_empty in Hi.
-  rewrite /temp /=.
+  destruct (ρ !! n) as [r|] eqn: Hn; rewrite Hn in Hi; last by rewrite lookup_empty in Hi.
+  rewrite /points_to_var /=.
   iDestruct "Hi" as (q) "Hi".
-  iAssert (|==> env_auth (set_temp ρ n i v') ∗ stack_frag n q q ∅ {[i := v']}) with "[-]" as ">($ & $)"; last done.
+  iAssert (|==> env_auth (set_var ρ n i v') ∗ stack_frag n q q {[i := v']})%I with "[-]" as ">($ & $)"; last done.
   rewrite -own_op; iApply (own_update_2 with "Hr Hi").
-  rewrite /set_temp.
-  destruct ρ as (?, s); rewrite Hn /=.
-  apply prod_update; first done.
-  rewrite /= !fmap_insert.
+  rewrite /set_var Hn /= !fmap_insert.
   eapply auth_update, (gmap.singleton_local_update(A := fixed_fracR frameR)).
   { rewrite lookup_fmap Hn //. }
   apply prod_local_update; simpl.
@@ -126,15 +129,12 @@ Lemma stack_frag_join : forall n q0 q0' q1 q2 r1 r2,
   stack_frag n q0 q1 r1 ∗ stack_frag n q0' q2 r2 ⊢ ⌜q0 = q0' ∧ r1 ##ₘ r2⌝ ∧ stack_frag n q0 (q1 + q2)%Qp (r1 ∪ r2).
 Proof.
   intros.
-  rewrite /stack_frag -own_op -cmra.pair_op -auth_frag_op gmap.singleton_op -!cmra.pair_op.
-  iIntros "H"; iDestruct (own_valid with "H") as %(_ & (Hq & _ & Hv & Ht)%auth_frag_valid_1%gmap.singleton_valid); simpl in *.
+  rewrite /stack_frag -own_op -auth_frag_op gmap.singleton_op -!cmra.pair_op.
+  iIntros "H"; iDestruct (own_valid with "H") as %(Hq & _ & Hr)%auth_frag_valid_1%gmap.singleton_valid; simpl in *.
   apply to_agree_op_inv_L in Hq as ->; rewrite agree_idemp !map_fmap_union.
-  assert (ve1 ##ₘ ve2).
-  { intros i; specialize (Hv i); rewrite gmap.lookup_op !lookup_fmap in Hv.
-    destruct (ve1 !! i)%stdpp, (ve2 !! i)%stdpp; done. }
-  assert (te1 ##ₘ te2).
-  { intros i; specialize (Ht i); rewrite gmap.lookup_op !lookup_fmap in Ht.
-    destruct (te1 !! i)%stdpp, (te2 !! i)%stdpp; done. }
+  assert (r1 ##ₘ r2).
+  { intros i; specialize (Hr i); rewrite gmap.lookup_op !lookup_fmap in Hr.
+    destruct (r1 !! i), (r2 !! i); done. }
   rewrite !gmap.gmap_op_union; auto; by apply map_disjoint_fmap.
 Qed.
 
@@ -143,11 +143,11 @@ Lemma stack_frag_split : forall n q0 q1 q2 r1 r2, r1 ##ₘ r2 →
   stack_frag n q0 q1 r1 ∗ stack_frag n q0 q2 r2.
 Proof.
   intros.
-  rewrite /stack_frag -own_op -cmra.pair_op -auth_frag_op gmap.singleton_op -!cmra.pair_op agree_idemp.
+  rewrite /stack_frag -own_op -auth_frag_op gmap.singleton_op -!cmra.pair_op agree_idemp.
   rewrite !map_fmap_union !gmap.gmap_op_union; auto; by apply map_disjoint_fmap.
 Qed.
 
-Lemma vars_equiv : forall lt lv n, length lt = length lv → list_norepet lt →
+Lemma vars_equiv : forall lt lv n, length lt = length lv → NoDup lt →
   ([∗ list] i;v ∈ lt;lv, points_to_var i v n) ⊣⊢ if decide (length lt = O) then emp else
   ∃ q : frac, stack_frag n q (pos_to_Qp (Pos.of_nat (length lt)) * q)%Qp (list_to_map (zip lt lv)).
 Proof.
@@ -160,7 +160,7 @@ Proof.
   iSplit.
   - iIntros "((% & H) & Hrest)".
     iExists q; iDestruct "Hrest" as (q') "Hrest".
-    iDestruct (stack_frag_join with "[$H $Hrest]") as ((<- & ? & _)) "H".
+    iDestruct (stack_frag_join with "[$H $Hrest]") as ((<- & ?)) "H".
     rewrite -insert_union_singleton_l.
     replace (pos_to_Qp (Pos.of_nat (S (base.length lt)))) with (1 + pos_to_Qp (Pos.of_nat (base.length lt)))%Qp.
     rewrite Qp.mul_add_distr_r Qp.mul_1_l //.
@@ -170,10 +170,9 @@ Proof.
     rewrite bi.sep_exist_r; iExists q.
     rewrite bi.sep_exist_l; iExists q.
     iApply stack_frag_split.
-    { done. }
     { apply map_disjoint_singleton_l_2.
       rewrite not_elem_of_list_to_map_1 //.
-      intros ((?, ?) & ? & ?%elem_of_zip_l%elem_of_list_In)%elem_of_list_fmap_2; simpl in *; congruence. }
+      intros ((?, ?) & ? & ?%elem_of_zip_l)%elem_of_list_fmap_2; simpl in *; congruence. }
     rewrite -insert_union_singleton_l.
     replace (pos_to_Qp (Pos.of_nat (S (length lt)))) with (1 + pos_to_Qp (Pos.of_nat (length lt)))%Qp.
     rewrite Qp.mul_add_distr_r Qp.mul_1_l //.
@@ -183,7 +182,7 @@ Qed.
 
 Definition alloc_vars r n (ρ : env_state) := <[n := r]>ρ.
 
-Lemma env_to_environ_alloc : forall ve te n ρ, env_to_environ (alloc_vars r n ρ) n = r.
+Lemma env_to_environ_alloc : forall r n ρ, env_to_environ (alloc_vars r n ρ) n = r.
 Proof.
   intros; rewrite /env_to_environ /alloc_vars lookup_insert //.
 Qed.
@@ -193,12 +192,11 @@ Lemma env_alloc : forall ρ n r, ρ !! n = None →
 Proof.
   intros.
   rewrite /env_auth /stack_frag -own_op; apply own_update.
-  apply prod_update; simpl; first reflexivity.
   rewrite fmap_insert.
   apply auth_update_alloc, (gmap.alloc_singleton_local_update(A := fixed_fracR frameR)).
   * rewrite lookup_fmap H //.
-  * split3; try done; simpl.
-    split; intros i; rewrite /= lookup_fmap; destruct (_ !! i)%stdpp; done.
+  * split; [|split]; try done; simpl.
+    intros i; rewrite /= lookup_fmap; destruct (_ !! i); done.
 Qed.
 
 Lemma env_to_environ_dealloc : forall n1 n2 ρ, n1 ≠ n2 → env_to_environ (delete n1 ρ) n2 = env_to_environ ρ n2.
@@ -211,7 +209,6 @@ Lemma env_dealloc : forall ρ n q r,
 Proof.
   intros.
   rewrite /env_auth /stack_frag -own_op; apply own_update.
-  apply prod_update; simpl; first reflexivity.
   rewrite fmap_delete.
   apply auth_update_dealloc, (gmap.delete_singleton_local_update(A := fixed_fracR frameR)), _.
 Qed.
