src/imp_notation.v
@@ -11,24 +11,22 @@ Delimit Scope stmt_scope with S.
 Declare Scope func_scope.
 Delimit Scope func_scope with F.
 
-Coercion LitInt : Z >-> base_lit.
+Coercion NumV : Z >-> val.
 
-Coercion Val : val >-> expr.
 Coercion Var : string >-> expr.
 
 Notation Load e := (UnOp DerefOp e).
 
 (* No scope for the values, does not conflict and scope is often not inferred
 properly. *)
-Notation "# l" := (LitV l%Z%V%stdpp) (at level 8, format "# l").
+Notation "# l" := (Num l%Z%stdpp) (at level 8, format "# l").
 
-Notation "()" := LitUnit : val_scope.
 Notation "! e" := (Load e%E) (at level 9, right associativity) : expr_scope.
 Notation "e1 + e2" := (BinOp PlusOp e1%E e2%E) : expr_scope.
 
-Notation "'Ref' x" := (Salloc x%binder) (at level 10) : stmt_scope.
+Notation "'Alloc' x" := (Salloc x%binder) (at level 10) : stmt_scope.
 Notation "e1 <- e2" := (Sstore e1%E e2%E) (at level 80) : stmt_scope.
-Notation "'Ret' e" := (Sreturn e%E) (at level 200) : stmt_scope.
+Notation "'Return' e" := (Sreturn e%E) (at level 200) : stmt_scope.
 Notation skip := Sskip.
 
 Notation "x <- f ( e )" := (Scall x%binder f%binder (@cons expr e%E nil))
@@ -49,7 +47,7 @@ Notation "s1 ;; s2" := (Sseq s1%S s2%S)
   format "'[' '[hv' '[' s1 ']' ;;  ']' '/' s2 ']'",
   right associativity) : stmt_scope.
 
-Notation "'fn' x  <{ s }> " := (Func [x%binder] s%S)
+Notation "'fn' x <{ s }> " := (Func [x%binder] s%S)
   (at level 200, x at level 1, s at level 200,
   format "'fn'  x  <{ '/  ' s '/' }> ") : func_scope.
 Notation "'fn' x y .. z <{ s }> " := (Func (cons x%binder (cons y%binder .. (cons z%binder nil) ..)) s%S)
@@ -72,7 +70,7 @@ Section NotationExample.
     Example fun_ex := 
         fn "x" "y" <{
             "x" <- #1 ;;
-            Ref "a" ;;
+            Alloc "a" ;;
             If "y" <{ skip }> <{ skip }> ;;
             While "y" <{
                 While "y" <{
@@ -81,8 +79,8 @@ Section NotationExample.
             }>;;
             "c" <- "f" (!"x") ;;
             "c" <- !"x" ;;
-            "d" <- "g" (#0, !"x"+!"y", "z", #()) ;;
-            Ret #0
+            "d" <- "g" (#0, !"x"+!"y", "z") ;;
+            Return #0
         }>.
 
 End NotationExample.
